%% LyX 2.0.6 created this file.  For more info, see http://www.lyx.org/.
%% Do not edit unless you really know what you are doing.
\documentclass[english]{article}
\usepackage[T1]{fontenc}
\usepackage[latin9]{inputenc}
\usepackage{amsmath}
\usepackage{babel}
\begin{document}

\title{Homework 2}


\author{Alexander Gould}

\maketitle
1. A and B are true. C is false.

3. Only A is true. (Although D should be...)

5A. There exists a student who spends more than five hours every weekday
in class.

5B. All students spend more than five hours every weekday in class.

5C. There exists a student who doesn't spend more than five hours
every weekday in class.

5D. No students spend more than five hours every weekday in class.

9A. $\exists x\left(P\left(x\right)\wedge Q\left(x\right)\right)$

9B. $\exists x\left(P\left(x\right)\wedge\neg Q\left(x\right)\right)$

9C. $\forall x\left(P\left(x\right)\vee Q\left(x\right)\right)$

9D. $\forall x\left(\neg P\left(x\right)\wedge\neg Q\left(x\right)\right)$

13. A is true because of the laws of addition, and 1 and 0 make B
and C true. D is false because the statement doesn't hold for negative
integers, yet the expression calls for all integers to fulfill it.

15. A is true, but B is false because $\sqrt{2}$ isn't an integer.
C is true, but D is false. (All squares of integers are positive.)

17A. $P\left(0\right)\vee P\left(1\right)\vee P\left(2\right)\vee P\left(3\right)\vee P\left(4\right)$

17C. $\neg P\left(0\right)\vee\neg P\left(1\right)\vee\neg P\left(2\right)\vee\neg P\left(3\right)\vee\neg P\left(4\right)$

17E. $\neg P\left(0\right)\wedge\neg P\left(1\right)\wedge\neg P\left(2\right)\wedge\neg P\left(3\right)\wedge\neg P\left(4\right)$

3A. There exists a sender and a recipient.

3B. There is someone who has emailed everybody.

3C. Everyone has sent an email to someone.

3D. (At least) One person has gotten an email from everyone.

3E. Everyone has recieved an email from someone.

3F. Everyone has emailed everyone.

9A. $\forall x\left(L\left(x,Jerry\right)\right)$

9B. $\forall x\exists y\left(L\left(x,y\right)\right)$

9C. $\exists y\forall x\left(L\left(x,y\right)\right)$

9D. $\neg\left(\exists x\forall y\left(L\left(x,y\right)\right)\right)$

9E. $\exists y\left(\neg\left(L\left(Lydia,y\right)\right)\right)$

29A. $P\left(1,1\right)\wedge P\left(1,2\right)\wedge P\left(1,3\right)\wedge P\left(2,1\right)\wedge P\left(2,2\right)\wedge P\left(2,3\right)\wedge P\left(3,1\right)\wedge P\left(3,2\right)\wedge P\left(3,3\right)$

29B. $P\left(1,1\right)\vee P\left(1,2\right)\vee P\left(1,3\right)\vee P\left(2,1\right)\vee P\left(2,2\right)\vee P\left(2,3\right)\vee P\left(3,1\right)\vee P\left(3,2\right)\vee P\left(3,3\right)$

29C. $\left(P\left(1,1\right)\wedge P\left(1,2\right)\wedge P\left(1,3\right)\right)\vee\left(P\left(2,1\right)\wedge P\left(2,2\right)\wedge P\left(2,3\right)\right)\vee\left(P\left(3,1\right)\wedge P\left(3,2\right)\wedge P\left(3,3\right)\right)$

29D. $\left(P\left(1,1\right)\vee P\left(1,2\right)\vee P\left(1,3\right)\right)\wedge\left(P\left(2,1\right)\vee P\left(2,2\right)\vee P\left(2,3\right)\right)\wedge\left(P\left(3,1\right)\vee P\left(3,2\right)\vee P\left(3,3\right)\right)$

30A. $\forall y\neg P(x,y)$

30B. $\exists x\forall y\neg\left(P\left(x,y\right)\right)$

30C. $\neg\exists y(Q(y)\wedge\forall x\neg R(x,y))\equiv\forall y\neg(Q(y)\wedge\forall x\neg R(x,y))\equiv\forall y(\neg Q(y)\vee\neg\forall x\neg R(x,y))\equiv\boxed{\forall y(\neg Q(y)\vee\exists xR(x,y))}$

30D. $\neg\exists y(\exists xR(x,y)\vee\forall xS(x,y))\equiv\forall y\neg(\exists xR(x,y)\vee\forall xS(x,y))\equiv\forall y(\neg\exists xR(x,y)\wedge\neg\forall xS(x,y))\equiv\boxed{\forall y(\forall x\neg R(x,y)\wedge\exists x\neg S(x,y))}$

30E. $\neg\exists y(\forall x\exists zT(x,y,z)\vee\exists x\forall zU(x,y,z))\equiv\forall y(\neg\forall x\exists zT(x,y,z)\wedge\neg\exists x\forall zU(x,y,z))\equiv\boxed{\forall y(\exists x\forall z\neg T(x,y,z)\wedge\forall x\exists z\neg U(x,y,z))}$

33A. $\neg\forall x\forall yP(x,y)\equiv\boxed{\exists x\exists y\neg P(x,y)}$

33B. $\text{\ensuremath{\neg\forall}}y\exists xP(x,y)\equiv\boxed{\exists y\forall x\neg P(x,y)}$

33C. $\neg\forall y\forall x(P(x,y)\vee Q(x,y))\equiv\exists y\exists x\neg(P(x,y)\vee Q(x,y))\equiv\boxed{\exists y\exists x(\neg P(x,y)\wedge\neg Q(x,y))}$

33D. $\text{\ensuremath{\neg}}(\exists x\exists y\neg P(x,y)\wedge\forall x\forall yQ(x,y))\equiv(\neg\exists x\exists y\neg P(x,y)\vee\neg\forall x\forall yQ(x,y))\equiv\boxed{(\forall x\forall yP(x,y)\vee\exists x\exists y\neg Q(x,y))}$

33E. $\neg\forall x(\exists y\forall zP(x,y,z)\wedge\exists z\forall yP(x,y,z))\equiv\exists x(\neg\exists y\forall zP(x,y,z)\vee\neg\exists z\forall yP(x,y,z))\equiv\boxed{\exists x(\forall y\exists z\neg P(x,y,z)\vee\forall z\exists\neg yP(x,y,z))}$

34. $x=\left\{ 4\right\} y=\left\{ 5\right\} z=\left\{ 4\right\} $would
make the statement true, $x=\left\{ 4\right\} y=\left\{ 5\right\} z=\left\{ 6\right\} $would
make it false.

35. $x=\left\{ 1,2,3\right\} y=\left\{ 1,2,3\right\} z=\left\{ 1,2,3\right\} w=\left\{ 4\right\} $would
make the statement true, $x=\left\{ 4\right\} y=\left\{ 4\right\} z=\left\{ 4\right\} w=\left\{ 4\right\} $
would make it false.
\end{document}
